+ 

+ If $A$ and $B$ are independent, then 
$P(A|B, C) = P(A|B^{c}, C) = P(A|C).$
$P(A|B, C^{c}) = P(A|B^{c}, C^{c}) = P(A|C^{c}).$

Thus, Simpson's Paradox does not hold.

+ If $A$ and $C$ are independent, then $P(A|B, C) < P(A|B^{c}, C) arrow.r.double P(A|B)
< P(A|B^{c}).$ Thus, Simpson's Paradox does not hold.

+ If $B$ and $C$ are independent, then
$P(A|B) = P(C)P(A|B, C) + P(C^{c})P(A|B, C^{c}).$
$P(A|B^{c}) = P(C)P(A|B^{c}, C) + P(C^{c})P(A|B^{c}, C^{c}).$

Since $P(A|B, C) > P(A|B^{c}, C)$ and $P(A|B, C^{c}) > P(A|B^{c}, C^{c})$, $P
(A|B) > P(A|B^{c})$, so Simpson's Paradox does not hold.