+ 

+ Since $P(W_{j} = y_{k})$
for $1 lt.eq k lt.eq N$ is $(binom(N-1, n-1))/(binom(N, n))(1)/(n) =
(n)/(N)(1)/(n) = (1)/(N)$,
$\text{E}(W_{j}) = (1)/(N)sum_(k=1)^(N)y_{k}.$
Thus,

$
\text{E}(\overline{W}) = (1)/(n)sum_(j=1)^(n)((1)/(N)sum_(k=1)^(N)y_{k}) 

= (1)/(N)sum_(k=1)^(N)y_{k} 

= \overline{y}
$

+ Since $\overline{W} = (1)/(n)sum_(j=1)^(N)(I_{j}y_{j})$ where $I_{j}$
is the
indicator variable for the $j$-th person being in the sample. Then, 

$
\text{E}(\overline{W}) = (1)/(n)sum_(j=1)^(N)(n)/(N)y_{j}

= (1)/(N)sum_(k=1)^(N)y_{k} 

= \overline{y}
$